rt refine: finish refillBudgetCheck_corres
Signed-off-by: Michael McInerney <m.mcinerney@unsw.edu.au>

proof/refine/ARM/SchedContextInv_R.thy
@@ -1580,9 +1580,15 @@ end
 global_interpretation handleOverrunLoopBody: typ_at_all_props' "handleOverrunLoopBody usage"
   by typ_at_props'
 
+global_interpretation handleOverrunLoop: typ_at_all_props' "handleOverrunLoop usage"
+  by typ_at_props'
+
+global_interpretation scheduleUsed: typ_at_all_props' "scheduleUsed scPtr new"
+  by typ_at_props'
+
 context begin interpretation Arch . (*FIXME: arch_split*)
 
-lemma unat_well_founded:
+lemma handle_overrun_loop_body_terminates_wf_helper:
   "wf {((r' :: ticks, s' :: 'a state), (r, s)). unat r' < unat r}"
   apply (insert wf_inv_image[where r="{(m, n). m < n}"
                                and f="\<lambda>(r :: ticks, s :: 'a state). unat r"])
@@ -1599,11 +1605,12 @@ lemma unat_well_founded:
   done
 
 lemma handle_overrun_loop_body_terminates:
-  "\<lbrakk>sc_at (cur_sc s) s; pred_map (\<lambda>cfg. \<forall>refill \<in> set (scrc_refills cfg). 0 < unat (r_amount refill))
+  "\<lbrakk>sc_at (cur_sc s) s;
+    pred_map (\<lambda>cfg. \<forall>refill \<in> set (scrc_refills cfg). 0 < unat (r_amount refill))
              (sc_refill_cfgs_of s) (cur_sc s);
     pred_map (\<lambda>cfg. scrc_refills cfg \<noteq> []) (sc_refill_cfgs_of s) (cur_sc s);
-    pred_map (\<lambda>cfg. refills_unat_sum (scrc_refills cfg) = unat (scrc_budget cfg)) (sc_refill_cfgs_of s)
-             (cur_sc s)\<rbrakk>
+    pred_map (\<lambda>cfg. refills_unat_sum (scrc_refills cfg) = unat (scrc_budget cfg))
+             (sc_refill_cfgs_of s) (cur_sc s)\<rbrakk>
    \<Longrightarrow> whileLoop_terminates (\<lambda>r s. the (head_time_buffer r s)) handle_overrun_loop_body usage s"
   (is "\<lbrakk>?P1 s; ?P2 s; ?P3 s; ?P4 s\<rbrakk> \<Longrightarrow> _")
   apply (rule_tac R="{((r' :: ticks, s' :: 'a state), (r, s)). unat r' < unat r}"
@@ -1611,62 +1618,49 @@ lemma handle_overrun_loop_body_terminates:
                in whileLoop_terminates_inv)
     apply simp
    prefer 2
-   apply (insert unat_well_founded)
-   apply simp
-  apply (intro hoare_vcg_conj_lift_pre_fix)
-apply (rule_tac f=cur_sc in hoare_lift_Pf2)
-apply wpsimp
-apply wpsimp
-apply (rule_tac f=cur_sc in hoare_lift_Pf2)
- apply (wpsimp wp: handle_overrun_loop_body_non_zero_refills)
-apply wpsimp
-apply (rule_tac f=cur_sc in hoare_lift_Pf2)
-apply wpsimp
-apply wpsimp
-apply (rule_tac f=cur_sc in hoare_lift_Pf2)
-apply (wpsimp wp: handle_overrun_loop_body_refills_unat_sum_equals_budget)
-apply wpsimp
-apply clarsimp
-apply wpsimp
-apply wpsimp
-apply (clarsimp simp: handle_overrun_loop_body_def)
-apply wpsimp
-apply (subst unat_sub)
-apply (prop_tac "sc_at (cur_sc sa) sa")
-apply (clarsimp simp: sc_at_ppred_def obj_at_def is_sc_obj_def vs_all_heap_simps
-split: Structures_A.kernel_object.splits)
-apply (frule_tac usage=r and s=sa in head_time_buffer_simp)
-apply (clarsimp simp: sc_at_ppred_def obj_at_def is_sc_obj_def vs_all_heap_simps
-split: Structures_A.kernel_object.splits)
-apply (clarsimp simp: sc_at_ppred_def obj_at_def is_sc_obj_def vs_all_heap_simps
-split: Structures_A.kernel_object.splits)
-apply (frule_tac x="refill_hd sc" in bspec)
+   apply (fastforce simp: handle_overrun_loop_body_terminates_wf_helper)
+  apply (rename_tac r s')
+  apply (intro hoare_vcg_conj_lift_pre_fix; (solves wpsimp)?)
+      apply (rule_tac f=cur_sc in hoare_lift_Pf2)
+       apply wpsimp
+      apply wpsimp
+     apply (rule_tac f=cur_sc in hoare_lift_Pf2)
+      apply (wpsimp wp: handle_overrun_loop_body_non_zero_refills)
+     apply wpsimp
+    apply (rule_tac f=cur_sc in hoare_lift_Pf2)
+     apply wpsimp
+    apply wpsimp
+   apply (rule_tac f=cur_sc in hoare_lift_Pf2)
+    apply (wpsimp wp: handle_overrun_loop_body_refills_unat_sum_equals_budget)
+   apply wpsimp
+  apply (wpsimp simp: handle_overrun_loop_body_def)
+  apply (rename_tac sc n)
+  apply (subst unat_sub)
+   apply (prop_tac "sc_at (cur_sc s') s'", simp)
+   apply (frule_tac usage=r and s=s' in head_time_buffer_simp)
+   apply (clarsimp simp: sc_at_ppred_def obj_at_def)
+  apply (clarsimp simp: obj_at_def vs_all_heap_simps)
+  apply (frule_tac x="refill_hd sc" in bspec, fastforce)
+  apply (prop_tac "0 < unat r")
+   apply (prop_tac "sc_at (cur_sc s') s'")
+    apply (clarsimp simp: obj_at_def is_sc_obj_def)
+   apply (frule_tac usage=r and s=s' in head_time_buffer_simp)
+   apply (clarsimp simp: sc_at_ppred_def obj_at_def)
+   apply (frule_tac x="refill_hd sc" in bspec, fastforce)
+   apply (fastforce simp: word_le_nat_alt)
   apply fastforce
-apply (prop_tac "0 < unat r")
-apply (prop_tac "sc_at (cur_sc sa) sa")
-apply (clarsimp simp: sc_at_ppred_def obj_at_def is_sc_obj_def vs_all_heap_simps
-split: Structures_A.kernel_object.splits)
-
-apply (frule_tac usage=r and s=sa in head_time_buffer_simp)
-apply (clarsimp simp: sc_at_ppred_def obj_at_def is_sc_obj_def vs_all_heap_simps
-split: Structures_A.kernel_object.splits)
-apply (frule_tac x="refill_hd sc" in bspec)
-  apply force
-apply (rule_tac y="unat (r_amount (refill_hd sc))" in less_le_trans)
-  apply fastforce
-apply (clarsimp simp: word_le_nat_alt)
-  apply linarith
-done
+  done
 
 lemma handleOverrunLoop_corres:
   "usage = usage' \<Longrightarrow>
-    corres (=) (\<lambda>s. sc_at (cur_sc s) s \<and> is_active_sc2 (cur_sc s) s \<and> pspace_aligned s
-                   \<and> pspace_distinct s \<and> valid_objs s
+   corres (=) (\<lambda>s. sc_at (cur_sc s) s \<and> is_active_sc2 (cur_sc s) s
+                   \<and> pspace_aligned s \<and> pspace_distinct s
+                   \<and> valid_objs s
                    \<and> pred_map (\<lambda>cfg. scrc_refills cfg \<noteq> []) (sc_refill_cfgs_of s) (cur_sc s)
-                   \<and>  pred_map (\<lambda>cfg. \<forall>refill\<in>set (scrc_refills cfg). 0 < unat (r_amount refill)) (sc_refill_cfgs_of s)
-                (cur_sc s)
-                   \<and>  pred_map (\<lambda>cfg. refills_unat_sum (scrc_refills cfg) = unat (scrc_budget cfg)) (sc_refill_cfgs_of s)
-                (cur_sc s))
+                   \<and> pred_map (\<lambda>cfg. \<forall>refill\<in>set (scrc_refills cfg). 0 < unat (r_amount refill))
+                               (sc_refill_cfgs_of s) (cur_sc s)
+                   \<and> pred_map (\<lambda>cfg. refills_unat_sum (scrc_refills cfg) = unat (scrc_budget cfg))
+                               (sc_refill_cfgs_of s) (cur_sc s))
               valid_objs'
               (handle_overrun_loop usage)
               (handleOverrunLoop usage')"
@@ -1681,52 +1675,318 @@ lemma handleOverrunLoop_corres:
       apply (corressimp corres: handleOverrunLoopBody_corres)
      apply (wpsimp wp: handle_overrun_loop_body_no_fail)
      apply (clarsimp simp: vs_all_heap_simps)
-apply (intro hoare_vcg_conj_lift_pre_fix; (solves wpsimp)?)
- thm hoare_lift_Pf
- apply (rule hoare_weaken_pre)
- apply (rule_tac f=cur_sc in hoare_lift_Pf)
- apply wpsimp
- apply wpsimp
- apply wpsimp
- apply (rule hoare_weaken_pre)
- apply (rule_tac f=cur_sc in hoare_lift_Pf)
- apply wpsimp
- apply wpsimp
- apply wpsimp
- apply (rule hoare_weaken_pre)
- apply (rule_tac f=cur_sc in hoare_lift_Pf)
- apply wpsimp
- apply wpsimp
- apply wpsimp
-
-apply (rule hoare_weaken_pre)
-apply (rule_tac f=cur_sc in hoare_lift_Pf2)
-
-apply (wpsimp wp: handle_overrun_loop_body_non_zero_refills)
-apply wpsimp
-apply (clarsimp split: if_splits)
-apply (rule hoare_weaken_pre)
-apply (rule_tac f=cur_sc in hoare_lift_Pf2)
-
-apply (wpsimp wp: handle_overrun_loop_body_refills_unat_sum_equals_budget)
-apply wpsimp
-apply (clarsimp split: if_splits)
-
- apply (clarsimp simp: pred_conj_def)
- apply (intro hoare_vcg_conj_lift_pre_fix; (solves wpsimp)?)
- apply (wpsimp wp: handleOverrunLoopBody_valid_objs')
- apply (rule hoare_weaken_pre)
- apply (rule_tac f=ksCurSc in hoare_lift_Pf)
- apply wpsimp
- apply wpsimp
- apply wpsimp
- apply (rule hoare_weaken_pre)
- apply (rule_tac f=ksCurSc in hoare_lift_Pf)
- apply wpsimp
- apply wpsimp
- apply wpsimp
- apply (fastforce intro:  handle_overrun_loop_body_terminates)
+    apply (intro hoare_vcg_conj_lift_pre_fix; (solves wpsimp)?)
+        apply (rule hoare_weaken_pre)
+         apply (rule_tac f=cur_sc in hoare_lift_Pf2)
+          apply wpsimp
+         apply wpsimp
+        apply wpsimp
+       apply (rule hoare_weaken_pre)
+        apply (rule_tac f=cur_sc in hoare_lift_Pf2)
+         apply wpsimp
+        apply wpsimp
+       apply wpsimp
+      apply (rule hoare_weaken_pre)
+       apply (rule_tac f=cur_sc in hoare_lift_Pf2)
+        apply wpsimp
+       apply wpsimp
+      apply wpsimp
+     apply (rule hoare_weaken_pre)
+      apply (rule_tac f=cur_sc in hoare_lift_Pf2)
+       apply (wpsimp wp: handle_overrun_loop_body_non_zero_refills)
+      apply wpsimp
+     apply clarsimp
+    apply (rule hoare_weaken_pre)
+     apply (rule_tac f=cur_sc in hoare_lift_Pf2)
+      apply (wpsimp wp: handle_overrun_loop_body_refills_unat_sum_equals_budget)
+     apply wpsimp
+    apply clarsimp
+   apply (clarsimp simp: pred_conj_def)
+   apply (intro hoare_vcg_conj_lift_pre_fix; (solves wpsimp)?)
+     apply (wpsimp wp: handleOverrunLoopBody_valid_objs')
+    apply (rule hoare_weaken_pre)
+     apply (rule_tac f=ksCurSc in hoare_lift_Pf)
+      apply wpsimp
+     apply wpsimp
+    apply wpsimp
+   apply (rule hoare_weaken_pre)
+    apply (rule_tac f=ksCurSc in hoare_lift_Pf)
+     apply wpsimp
+    apply wpsimp
+   apply wpsimp
+  apply (fastforce intro:  handle_overrun_loop_body_terminates)
   done
+
+lemma handle_overrun_loop_is_active_sc[wp]:
+  "handle_overrun_loop usage \<lbrace>\<lambda>s. is_active_sc sc_ptr s\<rbrace>"
+  apply handle_overrun_loop_simple
+  done
+
+lemma get_refills_exs_valid[wp]:
+  "sc_at sc_ptr s \<Longrightarrow> \<lbrace>(=) s\<rbrace> get_refills sc_ptr \<exists>\<lbrace>\<lambda>r. (=) s\<rbrace>"
+  apply (clarsimp simp: get_refills_def)
+  apply (wpsimp wp: get_sched_context_exs_valid)
+   apply (erule sc_atD1)
+  apply simp
+  done
+
+lemma corres_when3:
+  "\<lbrakk>G = G'; G \<Longrightarrow> corres_underlying sr nf nf' dc P P' a c\<rbrakk>
+\<Longrightarrow> corres_underlying sr nf nf' dc P P' (when G a) (when G' c)"
+apply (frule corres_when2)
+  apply blast
+apply (fastforce simp: corres_underlying_def when_def)
+done
+
+definition
+  refill_budget_check :: "ticks \<Rightarrow> (unit, 'z::state_ext) s_monad"
+where
+  "refill_budget_check usage \<equiv> do
+     sc_ptr \<leftarrow> gets cur_sc;
+
+     robin \<leftarrow> is_round_robin sc_ptr;
+     assert (\<not>robin);
+
+     usage' \<leftarrow> handle_overrun_loop usage;
+
+     sc \<leftarrow> get_sched_context sc_ptr;
+
+     when (usage' > 0 \<and> r_time (hd (sc_refills sc)) < MAX_RELEASE_TIME) $ do
+\<comment> \<open>       sc \<leftarrow> get_sched_context sc_ptr;\<close>
+       used \<leftarrow> return \<lparr>r_time = r_time (hd (sc_refills sc)) + sc_period sc, r_amount = usage'\<rparr>;
+       set_refill_hd sc_ptr \<lparr>r_time = r_time (refill_hd sc) + usage',
+                             r_amount = r_amount (refill_hd sc) - usage'\<rparr>;
+       schedule_used sc_ptr used
+     od;
+
+     head_insufficient_loop sc_ptr
+   od"
+
+definition refillBudgetCheck where "refillBudgetCheck usage \<equiv>
+do scPtr <- getCurSc;
+   active <- scActive scPtr;
+   haskell_assert active [];
+   roundRobin <- isRoundRobin scPtr;
+   haskell_assert (\<not> roundRobin) [];
+   usage' <- handleOverrunLoop usage;
+   sc <- getSchedContext scPtr;
+   when (0 < usage' \<and> rTime (refillHd sc) < maxReleaseTime) $
+   do
+      used <- return (Refill (rTime (refillHd sc) + scPeriod sc) usage');
+      setRefillHd scPtr (Refill (rTime (refillHd sc) + usage') (rAmount (refillHd sc) - usage'));
+      scheduleUsed scPtr used
+   od;
+   headInsufficientLoop scPtr
+od"
+
+lemma update_refill_hd_is_active_sc2[wp]:
+  "update_refill_hd sc_ptr f \<lbrace>is_active_sc2 sc_ptr'\<rbrace>"
+  apply (clarsimp simp: update_refill_hd_def)
+  apply (wpsimp wp: update_sched_context_wp)
+  apply (clarsimp simp: is_active_sc2_def obj_at_def opt_map_red)
+  done
+
+thm refillBudgetCheck_def[no_vars]
+lemma refillBudgtCheck_corres:
+  "usage = usage'
+   \<Longrightarrow> corres dc (\<lambda>s. sc_at (cur_sc s) s \<and> is_active_sc2 (cur_sc s) s \<and> valid_refills (cur_sc s) s
+                      \<and> \<not> round_robin (cur_sc s) s
+                      \<and> pspace_aligned s \<and> pspace_distinct s
+                      \<and> valid_objs s)
+                 valid_objs'
+                 (refill_budget_check usage)
+                 (refillBudgetCheck usage')"
+  apply (rule_tac Q="\<lambda>s'. sc_at' (ksCurSc s') s'" in corres_cross_add_guard)
+   apply (fastforce intro: sc_at_cross simp: state_relation_def)
+  apply (rule_tac Q="\<lambda>s'. is_active_sc' (ksCurSc s') s'" in corres_cross_add_guard)
+   apply (fastforce intro: is_active_sc'_cross simp: state_relation_def)
+  apply (clarsimp simp: refill_budget_check_def refillBudgetCheck_def set_refill_hd_def)
+  apply (rule corres_split'[rotated 2, OF gets_sp getCurSc_sp])
+   apply (corressimp corres: getCurSc_corres)
+  apply (rule corres_symb_exec_r[rotated, OF scActive_sp]; (solves \<open>wpsimp simp: scActive_def\<close>)?)
+  apply (rule corres_symb_exec_r[rotated, OF assert_sp]; (solves wpsimp)?)
+   apply (wpsimp wp: no_fail_assert simp: is_active_sc'_def opt_map_red obj_at_simps)
+  apply (rule corres_split'[rotated 2, OF is_round_robin_sp isRoundRobin_sp])
+   apply (corressimp corres: isRoundRobin_corres)
+  apply (rule corres_symb_exec_l[rotated, OF _  assert_sp]; (solves wpsimp)?)
+  apply (rule_tac F="\<not>roundRobin" in corres_req)
+   apply clarsimp
+  apply (rule corres_symb_exec_r[rotated, OF assert_sp]; (solves wpsimp)?)
+  apply (rule_tac Q="\<lambda>usage' s. pspace_aligned s \<and> pspace_distinct s \<and> sc_at (cur_sc s) s
+                           \<and> is_active_sc (cur_sc s) s \<and> valid_objs s
+                           \<and> pred_map (\<lambda>cfg. refills_unat_sum (scrc_refills cfg) = unat (scrc_budget cfg))
+                                       (sc_refill_cfgs_of s) (cur_sc s)
+                           \<and> pred_map (\<lambda>cfg. MIN_BUDGET \<le> scrc_budget cfg)
+                                       (sc_refill_cfgs_of s) (cur_sc s)
+                           \<and> sc_ptr = cur_sc s
+\<and> (pred_map (\<lambda>cfg. r_time (hd (scrc_refills cfg)) < MAX_RELEASE_TIME)
+                                            (sc_refill_cfgs_of s) (cur_sc s)
+                                   \<longrightarrow> pred_map (\<lambda>cfg. usage' < r_amount (hd (scrc_refills cfg)))
+                                                (sc_refill_cfgs_of s) (cur_sc s))
+                           \<and> pred_map (\<lambda>cfg. scrc_refills cfg \<noteq> [])
+                                       (sc_refill_cfgs_of s) (cur_sc s)"
+               and Q'="\<lambda>_ s'. valid_objs' s' \<and> active_sc_at' (ksCurSc s') s' \<and> scPtr = ksCurSc s'"
+               in corres_split')
+apply (corressimp corres: handleOverrunLoop_corres)
+apply (fastforce intro: valid_refills_refills_unat_sum_equals_budget
+simp: vs_all_heap_simps cfg_valid_refills_def round_robin_def sp_valid_refills_def)
+
+defer
+
+apply (clarsimp simp: pred_conj_def)
+  apply (intro hoare_vcg_conj_lift_pre_fix; (solves wpsimp)?)
+apply (rule_tac f=cur_sc in hoare_lift_Pf2)
+apply wpsimp
+apply wpsimp
+apply (rule_tac f=cur_sc in hoare_lift_Pf2)
+apply wpsimp
+apply (simp add: is_active_sc_rewrite)
+apply wpsimp
+apply (rule_tac f=cur_sc in hoare_lift_Pf2)
+apply (wpsimp wp: handle_overrun_loop_refills_unat_sum_equals_budget)
+apply (fastforce intro: valid_refills_refills_unat_sum_equals_budget
+simp: vs_all_heap_simps cfg_valid_refills_def round_robin_def sp_valid_refills_def)
+apply wpsimp
+apply handle_overrun_loop_simple
+
+   apply (clarsimp simp: handle_overrun_loop_def)
+   apply (wpsimp wp: valid_whileLoop[where I="\<lambda>_ s. pred_map \<top> (scs_of s) (cur_sc s)"])
+    apply (fastforce simp: head_time_buffer_true_imp_unat_buffer vs_all_heap_simps word_less_nat_alt
+                           word_le_nat_alt)
+   apply (clarsimp simp: vs_all_heap_simps)
+
+apply handle_overrun_loop_simple
+thm refill_budget_check_valid_refills
+  apply (intro hoare_vcg_conj_lift_pre_fix; (solves wpsimp)?)
+apply (wpsimp wp: handleOverrunLoop_valid_objs')
+apply (clarsimp simp: active_sc_at'_def obj_at_simps)
+apply (rule_tac f=ksCurSc in hoare_lift_Pf2)
+apply wpsimp
+apply (clarsimp simp: active_sc_at'_def obj_at_simps)
+apply wpsimp
+
+
+apply (clarsimp simp: get_refills_def)
+  apply (rule corres_split'[rotated 2, OF get_sched_context_sp get_sc_sp'])
+   apply (corressimp corres: get_sc_corres)
+apply (clarsimp simp: state_relation_def active_sc_at'_def obj_at_simps)
+
+  apply (rule_tac Q="\<lambda>_ s. pspace_aligned s \<and> pspace_distinct s \<and> sc_at (cur_sc s) s
+                           \<and> is_active_sc (cur_sc s) s \<and> valid_objs s
+                           \<and> pred_map (\<lambda>cfg. refills_unat_sum (scrc_refills cfg) = unat (scrc_budget cfg))
+                                       (sc_refill_cfgs_of s) (cur_sc s)
+                           \<and> pred_map (\<lambda>cfg. MIN_BUDGET \<le> scrc_budget cfg)
+                                       (sc_refill_cfgs_of s) (cur_sc s)
+                           \<and> scPtr = cur_sc s"
+               and Q'="\<lambda>_ s'. valid_objs' s' \<and> active_sc_at' (ksCurSc s') s' \<and> scPtr = ksCurSc s'" and r'=dc
+               in corres_split')
+defer
+apply (corressimp corres: headInsufficientLoop_corres)
+apply (intro conjI impI)
+prefer 2
+apply (fastforce intro: valid_refills_refills_unat_sum_equals_budget
+simp: vs_all_heap_simps cfg_valid_refills_def round_robin_def sp_valid_refills_def)
+apply (clarsimp simp: vs_all_heap_simps word_le_nat_alt)
+  apply (intro hoare_vcg_conj_lift_pre_fix; (solves wpsimp)?)
+apply (wpsimp simp: schedule_used_defs update_refill_hd_def set_refill_hd_def wp: update_sched_context_wp get_refills_wp)
+apply (clarsimp simp: obj_at_def is_sc_obj_def)
+
+apply (wpsimp simp: schedule_used_defs update_refill_hd_def wp: update_sched_context_wp get_refills_wp)
+apply (clarsimp simp: obj_at_def is_sc_obj_def vs_all_heap_simps)
+
+find_theorems schedule_used refills_unat_sum
+apply (rule_tac f=cur_sc in hoare_lift_Pf2)
+apply (wpsimp wp: schedule_used_refills_unat_sum update_sched_context_wp simp: update_refill_hd_def)
+
+apply (clarsimp simp: obj_at_def is_sc_obj_def vs_all_heap_simps)
+thm refills_unat_sum_append
+apply (clarsimp simp: refills_unat_sum_cons refills_unat_sum_append)
+apply (subst unat_sub)
+  apply fastforce
+apply (clarsimp simp: word_less_nat_alt)
+apply (drule less_imp_le)
+
+apply (prop_tac "refills_unat_sum [] = 0")
+apply (clarsimp simp: refills_unat_sum_def)
+apply clarsimp
+
+apply (case_tac "sc_refills sc"; clarsimp)
+apply (clarsimp simp: refills_unat_sum_cons refills_unat_sum_append)
+apply wpsimp
+apply schedule_used_simple
+
+find_theorems updateRefillHd valid_objs'
+
+
+apply (clarsimp simp: pred_conj_def)
+  apply (intro hoare_vcg_conj_lift_pre_fix; (solves wpsimp)?)
+
+apply (wpsimp simp: setRefillHd_def wp: updateRefillHd_valid_objs')
+
+apply (rule_tac f=ksCurSc in hoare_lift_Pf2)
+apply wpsimp
+apply (wpsimp simp: setRefillHd_def updateRefillHd_def)
+apply (wpsimp simp: setRefillHd_def updateRefillHd_def)
+find_theorems rTime rAmount
+
+
+
+apply (rule_tac F="rAmount (refillHd sca) = r_amount (refill_hd sc) \<and> rTime (refillHd sca) = r_time (refill_hd sc)"
+in corres_req)
+apply clarsimp
+apply (rule refill_hd_relation2)
+  apply fastforce
+apply (clarsimp simp: vs_all_heap_simps obj_at_def)
+apply (fastforce dest:sc_ko_at_valid_objs_valid_sc')
+
+apply (clarsimp simp: maxReleaseTime_equiv)
+thm corres_symb_exec_l
+thm corres_when2[no_vars]
+thm corres_when2[where G=True and G'=True, simplified]
+
+apply (rule corres_when3)
+  apply blast
+
+(*    apply (corressimp corres: get_sc_corres) *)
+apply (clarsimp simp: setRefillHd_def)
+(*
+
+
+
+
+
+  apply (rule corres_symb_exec_l[rotated, OF _  get_sched_context_sp]; (solves wpsimp)?)
+apply  (wpsimp wp: get_sched_context_exs_valid)
+apply (clarsimp simp: obj_at_def)
+  apply blast
+
+apply (wpsimp wp: get_sched_context_no_fail)
+apply (clarsimp simp: obj_at_def)
+apply (clarsimp simp: setRefillHd_def)
+ *)
+apply (rule corres_guard_imp)
+apply (clarsimp simp: setRefillHd_def)
+apply (rule corres_split[OF updateRefillHd_corres])
+apply simp
+apply (clarsimp simp: refill_map_def)
+apply (rule scheduleUsed_corres)
+apply simp
+apply (clarsimp simp: refill_map_def)
+apply (clarsimp simp: sc_relation_def)
+
+apply wpsimp
+
+apply (wpsimp wp: updateRefillHd_valid_objs')
+apply (clarsimp simp: is_active_sc_rewrite)
+apply clarsimp
+apply (intro conjI impI)
+apply (rule valid_objs'_valid_refills')
+apply simp
+apply (clarsimp simp: obj_at_simps)
+apply (clarsimp simp: active_sc_at'_def is_active_sc'_def obj_at_simps opt_map_red)
+
+apply (clarsimp simp: obj_at_simps)
+done
 
 (* FIXME RT: preconditions can be reduced, this is what is available at the call site: *)
 lemma invokeSchedControlConfigureFlags_corres:
